proof/invariant-abstract/AARCH64/ArchArch_AI.thy
@@ -438,7 +438,8 @@ lemma valid_arch_caps:
 
 lemma valid_asid_map':
   "valid_asid_map s \<Longrightarrow> valid_asid_map s'"
-  by (clarsimp simp: valid_asid_map_def)
+  by (clarsimp simp: valid_asid_map_def entry_for_asid_def obind_None_eq pool_for_asid_def s'_def
+                     entry_for_pool_def ko)
 
 lemma vspace_for_asid[simp]:
   "vspace_for_asid asid s' = vspace_for_asid asid s"
@@ -624,7 +625,8 @@ lemma valid_asid_map_asid_upd_strg:
    asid_pools_of s ap = Some Map.empty \<and>
    asid_table s asid = None \<longrightarrow>
    valid_asid_map (asid_table_update asid ap s)"
-  by (simp add: valid_asid_map_def)
+  by (simp add: valid_asid_map_def entry_for_asid_def obind_None_eq entry_for_pool_def
+                pool_for_asid_def)
 
 lemma valid_vspace_objs_asid_upd_strg:
   "valid_vspace_objs s \<and>
