proof/invariant-abstract/AARCH64/ArchKernelInit_AI.thy
@@ -390,9 +390,12 @@ lemma invs_A:
    apply (clarsimp simp: valid_arch_caps_def valid_asid_pool_caps_def unique_table_caps_def
                          caps_of_state_init_A_st_Null valid_table_caps_def unique_table_refs_def)
    apply (clarsimp simp: state_defs)
-  apply (clarsimp simp: valid_global_objs_def valid_kernel_mappings_def valid_asid_map_def)
+  apply (clarsimp simp: valid_global_objs_def valid_kernel_mappings_def)
   apply (rule conjI)
    apply (clarsimp simp: equal_kernel_mappings_def)
+  apply (rule conjI)
+   apply (clarsimp simp: valid_asid_map_def entry_for_asid_def init_A_st_def init_arch_state_def
+                         obind_def pool_for_asid_def)
   apply (simp add: pspace_in_kernel_window_init_A_st cap_refs_in_kernel_window_def
                    caps_of_state_init_A_st_Null valid_refs_def[unfolded cte_wp_at_caps_of_state])
   done
